Add inv_landin paradox

nola/iris/paradox.v
@@ -115,3 +115,155 @@ Module inv_fupd. Section inv_fupd.
     by iApply inv_bad_no.
   Qed.
 End inv_fupd. End inv_fupd.
+
+(** ** Paradox of the later-free invariant over an unguarded total Hoare triple,
+  via Landin's knot *)
+Module inv_landin. Section inv_landin.
+  (** Separation logic *)
+  Context {PROP : bi} `{!BiAffine PROP}.
+
+  (** Binary mask *)
+  Context {mask : Type} (mask_empty mask_full : mask).
+  Local Notation "∅" := mask_empty. Local Notation "⊤" := mask_full.
+
+  (** Location, value, closed expression *)
+  Context {loc val expr : Type}.
+  Context (atomic : expr → Prop).
+
+  (** Points-to token *)
+  Context (pointsto : loc → val → PROP).
+  Local Notation "l ↦ v" := (pointsto l v) (at level 20) : bi_scope.
+
+  (** Total Hoare triple *)
+  Context (thoare : mask → expr → PROP → (val → PROP) → PROP).
+  Local Notation "[[{ P } ] ] e @ E [[{ Ψ } ] ]" := (thoare E e P%I Ψ%I)
+    (at level 20, format "'[hv' [[{  '[' P  ']' } ] ]  '/  ' e  '/' @  E  '/' [[{  '[hv' Ψ  ']' } ] ] ']'")
+    : bi_scope.
+  Hypothesis thoare_persistent : ∀{E e P Ψ},
+    Persistent ([[{ P }]] e @ E [[{ Ψ }]]).
+  Hypothesis thoare_pre : ∀{E e P Ψ} P',
+    (P ⊢ P') → [[{ P' }]] e @ E [[{ Ψ }]] ⊢ [[{ P }]] e @ E [[{ Ψ }]].
+  Hypothesis thoare_post : ∀{E e P Ψ} Ψ',
+    (∀ v, Ψ' v ⊢ Ψ v) → [[{ P }]] e @ E [[{ Ψ' }]] ⊢ [[{ P }]] e @ E [[{ Ψ }]].
+  Hypothesis thoare_frame : ∀{E e P Ψ R},
+    [[{ P }]] e @ E [[{ Ψ }]] ⊢ [[{ P ∗ R }]] e @ E [[{ λ v, Ψ v ∗ R }]].
+  Hypothesis thoare_exists : ∀{A E e Φ Ψ},
+    (∀ a : A, [[{ Φ a }]] e @ E [[{ Ψ }]]) ⊢ [[{ ∃ a, Φ a }]] e @ E [[{ Ψ }]].
+  Hypothesis thoare_pure : ∀{E e φ P Ψ},
+    (⌜φ⌝ → [[{ P }]] e @ E [[{ Ψ }]]) ⊢ [[{ ⌜φ⌝ ∗ P }]] e @ E [[{ Ψ }]].
+  Hypothesis thoare_self : ∀{E e Ψ}, ⊢
+    [[{ [[{ True }]] e @ E [[{ Ψ }]] }]] e @ E [[{ Ψ }]].
+  Hypothesis thoare_apply : ∀{E e Ψ} P, Persistent P →
+    P ∗ [[{ P }]] e @ E [[{ Ψ }]] ⊢ [[{ True }]] e @ E [[{ Ψ }]].
+
+  (** Expression with a variable *)
+  Context {expr_val : Type}.
+  (** Substitution *)
+  Context (subst_val : expr_val → val → expr).
+  Local Coercion subst_val : expr_val >-> Funclass.
+
+  Implicit Types (l : loc) (v : val) (ev : expr_val).
+
+  (** Location value *)
+  Context (locval : loc → val).
+  Local Coercion locval : loc >-> val.
+  (** Function value *)
+  Context (funval : expr → val).
+  Local Notation "λ(), e" := (funval e) (at level 90).
+
+  (** Nop *)
+  Context (nop : expr).
+  Hypothesis thoare_nop : ∀{P E}, ⊢ [[{ P }]] nop @ E [[{ λ _, P }]].
+  (** Sequential execution *)
+  Context (bind : expr → expr_val → expr).
+  Local Notation "e >>= ev" := (bind e ev) (at level 80, right associativity).
+  Hypothesis thoare_bind : ∀{E e ev P Ψ} Φ,
+    [[{ P }]] e @ E [[{ Φ }]] ∗ (∀ v, [[{ Φ v }]] ev v @ E [[{ Ψ }]]) ⊢
+      [[{ P }]] e >>= ev @ E [[{ Ψ }]].
+  Context (seq : expr → expr → expr).
+  Local Notation "e >> e'" := (seq e e') (at level 80, right associativity).
+  Hypothesis thoare_seq : ∀{E e e' P Ψ} Φ,
+    [[{ P }]] e @ E [[{ Φ }]] ∗ (∀ v, [[{ Φ v }]] e' @ E [[{ Ψ }]]) ⊢
+      [[{ P }]] e >> e' @ E [[{ Ψ }]].
+  (** Allocation *)
+  Context (ref : val → expr).
+  Hypothesis thoare_ref : ∀{E v}, ⊢
+    [[{ True }]] ref v @ E [[{ λ w, ∃ l, ⌜w = l⌝ ∗ l ↦ v }]].
+  (** Store *)
+  Context (store : loc → val → expr).
+  Local Notation "l <- v" := (store l v) (at level 20).
+  Hypothesis atomic_store : ∀{l v}, atomic (l <- v).
+  Hypothesis thoare_store : ∀{E l v w}, ⊢
+    [[{ l ↦ v }]] l <- w @ E [[{ λ _, l ↦ w }]].
+  (** Load *)
+  Context (load : loc → expr).
+  Local Notation "! l" := (load l) (at level 20).
+  Hypothesis atomic_load : ∀{l}, atomic (!l).
+  Hypothesis thoare_load : ∀{E l v}, ⊢
+    [[{ l ↦ v }]] !l @ E [[{ λ v', ⌜v' = v⌝ ∗ l ↦ v }]].
+  (** Function call *)
+  Context (call : expr_val).
+  Hypothesis thoare_call : ∀{E e P Ψ},
+    [[{ P }]] e @ E [[{ Ψ }]] ⊢ [[{ P }]] call (λ(), e) @ E [[{ Ψ }]].
+
+  (** Termination of [call] *)
+  Definition termin_call f : PROP :=
+    [[{ True }]] call f @ ⊤ [[{ λ _, True }]].
+  (** Bad proposition with an unguarded total Hoare triple *)
+  Definition bad l : PROP := ∃ f, l ↦ f ∗ termin_call f.
+
+  (** Later-free invariant on the bad proposition *)
+  Context (inv_bad : loc → PROP).
+  Hypothesis inv_bad_persistent : ∀{l}, Persistent (inv_bad l).
+  Hypothesis thoare_inv_bad_alloc : ∀{l e P Ψ},
+    [[{ inv_bad l ∗ P }]] e @ ⊤ [[{ Ψ }]] ⊢ [[{ bad l ∗ P }]] e @ ⊤ [[{ Ψ }]].
+  Hypothesis thoare_inv_bad_acc : ∀{l e P Ψ}, atomic e →
+    [[{ bad l ∗ P }]] e @ ∅ [[{ λ v, bad l ∗ Ψ v }]] ⊢
+      [[{ inv_bad l ∗ P }]] e @ ⊤ [[{ Ψ }]].
+
+  (** Bad call *)
+  Definition badcall l := !l >>= call.
+  (** Bad function value *)
+  Definition badfun l := λ(), badcall l.
+
+  (** Landin's knot *)
+  Definition landin_body l := l <- badfun l >> badcall l.
+  Context (landin_body' : expr_val).
+  Hypothesis landin_body_subst : ∀{l}, landin_body l = landin_body' l.
+  Definition landin := ref (λ(), nop) >>= landin_body'.
+
+  (** [badcall] terminates under [inv_bad] *)
+  Lemma thoare_badcall {l} : ⊢
+    [[{ inv_bad l }]] badcall l @ ⊤ [[{ λ _, True }]].
+  Proof.
+    iApply (thoare_bind termin_call). iSplit; last first.
+    { iIntros (f). iApply thoare_self. }
+    iApply (thoare_pre (inv_bad l ∗ True)); [by iIntros "$"|].
+    iApply thoare_inv_bad_acc; [by apply atomic_load|].
+    iApply (thoare_pre (bad l)); [by iIntros "[$ _]"|]. iApply thoare_exists.
+    iIntros (f).
+    iApply thoare_post; [|iApply thoare_frame; by iApply thoare_load].
+    iIntros (?) "[[-> $]#?]". by iSplit.
+  Qed.
+
+  (** Landin's knot is shown to terminate, which is contradictory because it
+    actually loops infinitely in the expected operational semantics *)
+  Lemma thoare_landin : ⊢ [[{ True }]] landin @ ⊤ [[{ λ _, True }]].
+  Proof.
+    iApply thoare_bind. iSplit; [iApply thoare_ref|]. iIntros (?).
+    iApply thoare_exists. iIntros (l). iApply thoare_pure. iIntros (->).
+    rewrite -landin_body_subst. iApply (thoare_pre (bad l)).
+    { iIntros "$". iApply thoare_call. iApply thoare_nop. }
+    iApply (thoare_pre (bad l ∗ True)); [by iIntros "$"|].
+    iApply thoare_inv_bad_alloc. iApply thoare_seq.
+    iSplit; [|iIntros (?); iApply thoare_badcall].
+    iApply (thoare_pre (inv_bad l ∗ inv_bad l)); [iIntros "[#? _]"; by iSplit|].
+    iApply thoare_inv_bad_acc; [by apply atomic_store|].
+    iApply (thoare_pre (∃ f, l ↦ f ∗ inv_bad l)); [by iIntros "[[%[$ _]]$]"|].
+    iApply thoare_exists. iIntros (g).
+    iApply thoare_post; [|iApply thoare_frame; by iApply thoare_store].
+    iIntros (?) "[$ #i]". iSplit; [|done]. iApply thoare_call.
+    iApply (thoare_apply (inv_bad l)). iSplit; [done|].
+    iApply thoare_badcall.
+  Qed.
+End inv_landin. End inv_landin.
